coaster

lunarlander/coaster.thy
@@ -70,7 +70,7 @@ consts Inv :: fform
 definition pre1 :: fform where
 "pre1 == (Real g[>] Real 0)
       [&](v[>]Real 0)
-      [&](v[**]2 [+] Real (2*g) [*] y [=]Real (2*g*yG))
+      [&](v[**]2 [+] Real (2*g) [*] y [=]Real(v0^2)[+]Real (2*g*yG))
       [&] (x[\<le>]Real x1 [&] x[\<ge>]Real x0 [&] y[\<le>] Real y1 [&] y[\<ge>] Real y0)
       [&]((Real dy0[\<le>]Real 0 [&] x[\<le>]Real x1 [&] x[\<ge>]Real x0 [&] y[\<le>] Real y1 [&] y[\<ge>] Real y0) 
         [\<longrightarrow>](v[**]2[\<ge>]Real vLo [&] v[**]2[\<le>]Real vHi [&] Real (dyLo*g)[\<le>] Real (-dy0*g)[&]Real (-dy0*g)[\<le>]Real (dyHi*g)[&] Real dx0[*]y [=] Real dy0[*]x [+] Real (dx0*c)))
@@ -82,15 +82,9 @@ definition pre1 :: fform where
 
 definition post1 :: fform where
 "post1 == (v[>]Real 0)
-      [&](v[**]2 [+] Real (2*g) [*] y [=]Real (2*g*yG))
+      [&](v[**]2 [+] Real (2*g) [*] y [=]Real(v0^2)[+]Real (2*g*yG))
       [&](x[\<le>]Real x1 [&] x[\<ge>]Real x0)
       [&](Real dx0[*]y [=] Real dy0[*]x [+] Real (dx0*c))"
-
-definition Inv1 :: fform where
-"Inv1 == (v[>]Real 0)
-      [&](v[**]2 [+] Real (2*g) [*] y [=]Real (2*g*yG))
-      [&]Real dx0[*]y [=] Real dy0[*]x [+] Real (dx0*c)"
-
 
 
 definition cons11 :: fform where
@@ -101,7 +95,7 @@ definition cons13 :: fform where
 "cons13 ==  (exeFlow(<[''parx'', ''pary'', ''parv'']: [(v[*]Real dx0),(v[*]Real dy0),(Real (-dy0*g))] && Inv & (x[\<le>]Real x1 [&] x[\<ge>]Real x0 [&] y[\<le>] Real y1 [&] y[\<ge>] Real y0)>) (Inv)  [\<longrightarrow>]  Inv )"
 lemma allcons1: "\<forall>s. (cons11[&]cons12 [&] cons13 ) s"
   apply (simp add: cons11_def cons12_def cons13_def  x_def y_def v_def pre1_def post1_def)
-  by (inv_check_oracle "g > 0 & dy0 <= 0 & parv > 0 & parv^2 + 2*g*pary - 2*g*yG = 0 & dx0*pary - dy0*parx - dx0*c = 0 ")
+  by (inv_check_oracle "g > 0 & dy0 <= 0 & parv > 0 & parv^2 + 2*g*pary -v0^2- 2*g*yG = 0 & dx0*pary - dy0*parx - dx0*c = 0 ")
 
 lemma linedown:"{pre1}
              <[''parx'', ''pary'', ''parv'']: [(v[*]Real dx0),(v[*]Real dy0),(Real (-dy0*g))] && Inv & (x[\<le>]Real x1 [&] x[\<ge>]Real x0 [&] y[\<le>] Real y1 [&] y[\<ge>] Real y0)>
@@ -132,7 +126,7 @@ apply (cut_tac allcons1)
 definition pre2 :: fform where
 "pre2 == (Real g[>] Real 0)
       [&](v[>]Real 0)
-      [&](v[**]2 [+] Real (2*g) [*] y [=]Real (2*g*yG))
+      [&](v[**]2 [+] Real (2*g) [*] y [=]Real(v0^2)[+]Real (2*g*yG))
       [&] (x[\<le>]Real x1 [&] x[\<ge>]Real x0 [&] y[\<le>] Real y1 [&] y[\<ge>] Real y0)
       [&]((Real dy0[\<ge>]Real 0 [&] x[\<le>]Real x1 [&] x[\<ge>]Real x0 [&] y[\<le>] Real y1 [&] y[\<ge>] Real y0) 
         [\<longrightarrow>](v[**]2[\<ge>]Real vLo [&] v[**]2[\<le>]Real vHi [&] Real (dyLo*g)[\<le>] Real (-dy0*g)[&]Real (-dy0*g)[\<le>]Real (dyHi*g)[&] Real dx0[*]y [=] Real dy0[*]x [+] Real (dx0*c)))
@@ -145,7 +139,7 @@ definition pre2 :: fform where
 
 definition post2 :: fform where
 "post2 == (v[>]Real 0)
-      [&](v[**]2 [+] Real (2*g) [*] y [=]Real (2*g*yG))
+      [&](v[**]2 [+] Real (2*g) [*] y [=]Real(v0^2)[+]Real (2*g*yG))
       [&]x[\<le>]Real x1 [&] x[\<ge>]Real x0
       [&]Real dx0[*]y [=] Real dy0[*]x [+] Real (dx0*c)
       "
@@ -158,7 +152,7 @@ definition cons23 :: fform where
 
 lemma allcons2: "\<forall>s. (cons21[&]cons22[&] cons23 ) s"
   apply (simp add: cons21_def cons22_def cons23_def  x_def y_def v_def a_def pre2_def post2_def)
-by (inv_check_oracle "parv*para^2 - 1 = 0 & parv^2 + 2*g*pary - 2*g*yG = 0 & parv > 0 & dx0*pary - dy0*parx -dx0*c = 0")
+by (inv_check_oracle "parv*para^2 - 1 = 0 & parv^2 + 2*g*pary -v0^2- 2*g*yG = 0 & parv > 0 & dx0*pary - dy0*parx -dx0*c = 0")
 
 
 
@@ -268,105 +262,879 @@ lemma lineup:"{pre2}
     done
   done
 definition pre3 :: fform where
-"pre3 == (Real g[\<ge>] Real 0)
+"pre3 == (Real g[>] Real 0)
       [&](v[>]Real 0)
-      [&](v[**]2 [+] Real (2*g) [*] y [=]Real (2*g*yG))
+      [&](v[**]2 [+] Real (2*g) [*] y [=]Real (v0^2)[+]Real (2*g*yG))
       [&]((Real dy0[\<le>]Real 0 [&] x[\<le>]Real x1 [&] x[\<ge>]Real x0 [&] y[\<le>] Real y0 [&] y[\<ge>] Real y1)
        [\<longrightarrow>](((x[-]Real cx)[**]2[+](y[-]Real cy)[**]2) [=] Real r [**]2 [&] x[\<ge>] Real cx[&] y[\<ge>] Real cy[&]v[**]2[\<ge>]Real vLo [&] v[**]2[\<le>]Real vHi [&] Real centLo[\<le>] Real cent[&]Real cent [\<le>]Real centHi [&] Real tanLo[\<le>]Real tan[&] Real tan[\<le>] Real tanHi))
       [&](Real dy0[\<le>]Real 0)
-      [&](dx[=](y[-]Real cy)[div]Real r)
-      [&](dy[=](Real cx[-]x)[div]Real r)
+      [&](dx[*]Real r [=](y[-]Real cy))
+      [&](dy[*]Real r [=](Real cx[-]x))
       [&](Real x1[>]Real x0)
       [&](Real y1[<]Real y0)
       [&](Real cy[\<le>]Real y1)
       [&](Real cx[\<le>]Real x0)
-      [&](Real r[>]Real 0) "
+      [&](Real r[>]Real 0) 
+      [&]((x[\<le>]Real x1 [&] x[\<ge>]Real x0 [&] y[\<le>] Real y0 [&] y[\<ge>] Real y1))"
 
 definition post3 :: fform where
-"post3 == (dx[=] (y[-]Real cy)[div]Real r)
-       [&](dy[=] (Real cx[-]x)[div]Real r)
-       [&](v[>]Real 0)
-       [&](v[**]2 [+] Real (2*g) [*] y [=]Real (2*g*yG))
-       [&](y[>]Real cy)
-       [&](((x[-]Real cx)[**]2[+](y[-]Real cy)[**]2) [=] Real r [**]2)"
+"post3 == (dx[*]Real r [=](y[-]Real cy))
+       [&](dy[*]Real r [=](Real cx[-]x))
+       [&](v[**]2 [+] Real (2*g) [*] y [=]Real(v0^2)[+]Real (2*g*yG))
+       [&](((x[-]Real cx)[**]2[+](y[-]Real cy)[**]2) [=] Real r [**]2)
+       [&](y[\<ge>]Real cy)"
+       
 
-definition Inv3 :: fform where
-"Inv3 == Inv"
+definition cons31 :: fform where
+"cons31 == pre3 [\<longrightarrow>] Inv"
+definition cons32 :: fform where
+"cons32 == Inv[&]close(x[\<le>]Real x1 [&] x[\<ge>]Real x0 [&] y[\<le>] Real y0 [&] y[\<ge>] Real y1)[\<longrightarrow>]post3"
+definition cons33 :: fform where
+"cons33 ==  (exeFlow(<[''parx'', ''pary'', ''parv'', ''pardx'',  ''pardy'']: [(v[*]dx),(v[*]dy),(dy[*]Real -g),((dy[*]v)[div]Real r),((Real 0[-]dx[*]v)[div]Real r)] && Inv & (x[\<le>]Real x1 [&] x[\<ge>]Real x0 [&] y[\<le>] Real y0 [&] y[\<ge>] Real y1)>) (Inv)  [\<longrightarrow>]  Inv )"
+lemma allcons3: "\<forall>s. (cons31[&]cons32[&]cons33 ) s"
+apply (simp add: cons31_def cons32_def cons33_def  x_def y_def v_def dx_def dy_def pre3_def post3_def)
+  by (inv_check_oracle
+   " r>0 &
+     pardx*r - pary + cy = 0 &
+     pardy*r - cx + parx = 0 &
+     y1 - cy >= 0 & x0 - cx >= 0 &
+     parv^2 + 2*g*pary -v0^2- 2*g*yG = 0 &
+     g > 0 & parv > 0 &
+     (parx-cx)^2+(pary-cy)^2-r^2 = 0"
+   "y1" "x0")
+
+
 
 
 lemma q1:"{pre3}
-         <[''x'', ''y'', ''v'', ''dx'', ''dy'']: [(v[*]dx),(v[*]dy),(dy[*]Real -g),((dy[*]v)[div]Real r),((Real 0[-]dx[*]v)[div]Real r)] && Inv & (x[\<le>]Real x1 [&] x[\<ge>]Real x0 [&] y[\<le>] Real y0 [&] y[\<ge>] Real y1)>
+         <[''parx'', ''pary'', ''parv'', ''pardx'', ''pardy'']: [(v[*]dx),(v[*]dy),(dy[*]Real -g),((dy[*]v)[div]Real r),((Real 0[-]dx[*]v)[div]Real r)] && Inv & (x[\<le>]Real x1 [&] x[\<ge>]Real x0 [&] y[\<le>] Real y0 [&] y[\<ge>] Real y1)>
           {post3;(elE 0 [[|]] (almost post3))}"
-  sorry
+  apply (rule ContinuousRuleGT )
+  apply auto
+       apply(simp add:pre3_def fAnd_def)
+      apply (cut_tac allcons3)
+      apply (simp add:cons31_def fAnd_def fImp_def)
+     apply (subgoal_tac "\<forall>s. cons32 s")
+      apply (simp add:cons32_def fImp_def )
+      apply (simp add:fAnd_def)
+     apply (cut_tac allcons3)
+     apply (simp add:fAnd_def )
+apply (cut_tac allcons3)
+    apply (simp add:cons33_def fAnd_def fImp_def)
+   apply (simp add:dOr_def)
+apply (subgoal_tac "\<forall>s. cons32 s")
+   apply (simp add:cons32_def fImp_def )
+   apply (simp add:dOr_def almost_def)
+ apply (cut_tac allcons3)
+  apply (simp add:fAnd_def )
+  done
+
+
+
 
 definition pre4 :: fform where
-"pre4 == (Real g[\<ge>] Real 0)
+"pre4 == (Real g[>] Real 0)
       [&](v[>]Real 0)
-      [&](v[**]2 [+] Real (2*g) [*] y [=]Real (2*g*yG))
+      [&](v[**]2 [+] Real (2*g) [*] y [=]Real (v0^2)[+]Real (2*g*yG))
       [&]((Real dy0[\<ge>]Real 0 [&] x[\<le>]Real x1 [&] x[\<ge>]Real x0 [&] y[\<le>] Real y0 [&] y[\<ge>] Real y1)
          [\<longrightarrow>](((x[-]Real cx)[**]2[+](y[-]Real cy)[**]2) [=] Real r [**]2 [&] x[\<ge>] Real cx[&] y[\<ge>] Real cy[&]v[**]2[\<ge>]Real vLo [&] v[**]2[\<le>]Real vHi [&] Real centLo[\<le>] Real cent[&]Real cent [\<le>]Real centHi [&] Real tanLo[\<le>]Real tan[&] Real tan[\<le>] Real tanHi))
       [&](Real dy0[\<ge>]Real 0)
-      [&](dx[=](Real cy[-]y)[div]Real r)
-      [&](dy[=](x[-]Real cx)[div]Real r)
+      [&](dx[*]Real r[=](Real cy[-]y))
+      [&](dy[*]Real r[=](x[-]Real cx))
       [&](Real x1[>]Real x0)
       [&](Real y1[<]Real y0)
       [&](Real r[>]Real 0)
       [&](Real cy[\<le>]Real y1)
       [&](Real cx[\<le>]Real x0)
-      [&]((x[\<le>]Real x1 [&] x[\<ge>]Real x0 [&] y[\<le>] Real y0 [&] y[\<ge>] Real y1)[\<longrightarrow>](v[**]2)[div]Real 2[>]Real g[*](Real y0[-]y))"
+      [&]((x[\<le>]Real x1 [&] x[\<ge>]Real x0 [&] y[\<le>] Real y0 [&] y[\<ge>] Real y1)[\<longrightarrow>](v[**]2)[div]Real 2[>]Real g[*](Real y0[-]y))
+      [&](x[\<le>]Real x1 [&] x[\<ge>]Real x0 [&] y[\<le>] Real y0 [&] y[\<ge>] Real y1)"
       
 definition post4 :: fform where
-"post4 == (dx[=](Real cy[-]y)[div]Real r)
-       [&](dy[=](x[-]Real cx)[div]Real r)
+"post4 == (dx[*]Real r[=](Real cy[-]y))
+       [&](dy[*]Real r[=](x[-]Real cx))
        [&](v[>]Real 0)
-       [&](v[**]2 [+] Real (2*g) [*] y [=]Real (2*g*yG))
-       [&](y[>]Real cy)
+       [&](v[**]2 [+] Real (2*g) [*] y [=]Real (v0^2)[+]Real (2*g*yG))
+       [&](y[\<ge>]Real cy)
        [&](((x[-]Real cx)[**]2[+](y[-]Real cy)[**]2) [=] Real r [**]2)"
 
-definition Inv4 :: fform where
-"Inv4 == Inv"
+
+definition cons41 :: fform where
+"cons41 == pre4[&](v[*](a[**]2)[=]Real 1) [\<longrightarrow>] Inv"
+definition cons42 :: fform where
+"cons42 == Inv[&]close(x[\<le>]Real x1 [&] x[\<ge>]Real x0 [&] y[\<le>] Real y0 [&] y[\<ge>] Real y1)[\<longrightarrow>](post4[&](v[*](a[**]2)[=]Real 1))"
+definition cons43 :: fform where
+"cons43 == (exeFlow(<[''parx'', ''pary'', ''parv'', ''pardx'',  ''pardy'', ''para'']: [(v[*]dx),(v[*]dy),(dy[*](Real -g)),((Real 0[-]dy[*]v)[div]Real r),((dx[*]v)[div]Real r),(((a[*]dy[*]Real g)[div](Real 2))[div]v)] && Inv & (x[\<le>]Real x1 [&] x[\<ge>]Real x0 [&] y[\<le>] Real y0 [&] y[\<ge>] Real y1)>) (Inv)  [\<longrightarrow>]  Inv )"
 
 
+lemma allcons4: "\<forall>s. (cons41[&]cons42[&]cons43 ) s"
+  apply (simp add: cons41_def cons42_def cons43_def pre4_def post4_def x_def y_def v_def dx_def dy_def a_def)
+  by (inv_check_oracle "
+       parv*(para^2)- 1  =0 & 
+       parv > 0 & 
+       pardx*r + pary - cy = 0 &
+       pardy*r + cx - parx = 0 &
+       parv^2 + 2*g*pary -v0^2- 2*g*yG = 0 &
+      (parx-cx)^2+(pary-cy)^2-r^2 = 0 &
+       y1 - cy >= 0" "y1")
+
+
+
+lemma q1cwle:"{pre4[&](v[*](a[**]2)[=]Real 1)}
+         <[''parx'', ''pary'', ''parv'', ''pardx'',  ''pardy'', ''para'']: [(v[*]dx),(v[*]dy),(dy[*](Real -g)),((Real 0[-]dy[*]v)[div]Real r),((dx[*]v)[div]Real r),(((a[*]dy[*]Real g)[div](Real 2))[div]v)] && Inv & (x[\<le>]Real x1 [&] x[\<ge>]Real x0 [&] y[\<le>] Real y0 [&] y[\<ge>] Real y1)>
+          {post4[&](v[*](a[**]2)[=]Real 1);(elE 0 [[|]] (almost (post4[&](v[*](a[**]2)[=]Real 1))))}"
+   apply (rule ContinuousRuleGT )
+  apply auto
+       apply(simp add:pre4_def fAnd_def)
+      apply (cut_tac allcons4)
+      apply (simp add:cons41_def fAnd_def fImp_def)
+     apply (subgoal_tac "\<forall>s. cons42 s")
+      apply (simp add:cons42_def fImp_def )
+      apply (simp add:fAnd_def)
+     apply (cut_tac allcons4)
+     apply (simp add:fAnd_def )
+apply (cut_tac allcons4)
+    apply (simp add:cons43_def fAnd_def fImp_def)
+   apply (simp add:dOr_def)
+apply (subgoal_tac "\<forall>s. cons42 s")
+   apply (simp add:cons42_def fImp_def )
+   apply (simp add:dOr_def almost_def)
+ apply (cut_tac allcons4)
+  apply (simp add:fAnd_def )
+  done
 lemma q1cw:"{pre4}
-         <[''x'', ''y'', ''v'', ''dx'', ''dy'']: [(v[*]dx),(v[*]dy),(dy[*]Real -g),((Real 0[-]dy[*]v)[div]Real r),((dx[*]v)[div]Real r)] && Inv & (x[\<le>]Real x1 [&] x[\<ge>]Real x0 [&] y[\<le>] Real y0 [&] y[\<ge>] Real y1)>
-          {post4;(elE 0 [[|]] (almost post4))}"
-  sorry
-
+         <[''parx'', ''pary'', ''parv'', ''pardx'',  ''pardy'']: [(v[*]dx),(v[*]dy),(dy[*](Real -g)),((Real 0[-]dy[*]v)[div]Real r),((dx[*]v)[div]Real r)] && Inv & (x[\<le>]Real x1 [&] x[\<ge>]Real x0 [&] y[\<le>] Real y0 [&] y[\<ge>] Real y1)>
+          {post4;(elE 0 [[|]] (almost (post4)))}"
+apply (rule GhostRule[where w="''para''"
+                          and F="(((a[*]dy[*]Real g)[div](Real 2))[div]v)"
+                          and pre="pre4[&](v[*](a[**]2)[=]Real 1)"
+                          and post="post4[&](v[*](a[**]2)[=]Real 1)"
+                          and HF="(elE 0)[[|]]almost (post4[&](v[*](a[**]2)[=]Real 1))"])
+         apply auto
+  apply(simp add:pre4_def fAnd_def fGreaterEqual_def fLessEqual_def fOr_def fImp_def fEqual_def fLess_def fGreater_def fNot_def not_in_fform_def x_def y_def v_def dx_def dy_def)
+   apply(simp add:post4_def fAnd_def fGreaterEqual_def fLessEqual_def fOr_def fImp_def fEqual_def fLess_def fGreater_def fNot_def not_in_fform_def x_def y_def v_def dx_def dy_def) 
+  apply(simp add:dOr_def post4_def fAnd_def fGreaterEqual_def fLessEqual_def fOr_def fImp_def fEqual_def fLess_def fGreater_def fNot_def not_in_dform_def x_def y_def v_def dx_def dy_def almost_def)
+  apply(subgoal_tac "{pre4[&](v[*](a[**]2)[=]Real 1)}
+         <[''parx'', ''pary'', ''parv'', ''pardx'',  ''pardy'', ''para'']: [(v[*]dx),(v[*]dy),(dy[*](Real -g)),((Real 0[-]dy[*]v)[div]Real r),((dx[*]v)[div]Real r),(((a[*]dy[*]Real g)[div](Real 2))[div]v)] && Inv & (x[\<le>]Real x1 [&] x[\<ge>]Real x0 [&] y[\<le>] Real y0 [&] y[\<ge>] Real y1)>
+          {post4[&](v[*](a[**]2)[=]Real 1);(elE 0 [[|]] (almost (post4[&](v[*](a[**]2)[=]Real 1))))}")
+  apply(simp add: dOr_def)
+     apply (rule q1cwle)
+  subgoal for s
+  proof -
+    have not_a: "not_in_fform ''para'' pre4"
+      by (simp add:pre4_def fAnd_def fGreaterEqual_def fLessEqual_def fOr_def fImp_def fEqual_def fLess_def fGreater_def fNot_def not_in_fform_def x_def y_def v_def dx_def dy_def)
+    have eq: "pre4 (\<lambda>y. if y \<noteq> ''para'' then s y else 1 / sqrt (evalE v s)) \<longleftrightarrow> pre4 s"
+      by (simp add: not_in_fform_update[OF not_a])
+    show ?thesis
+      apply (rule exI[where x="1/sqrt(evalE v s)"])
+      apply (auto simp add: eq fAnd_def fGreaterEqual_def fLessEqual_def fOr_def fImp_def fEqual_def fLess_def fGreater_def fNot_def  x_def y_def v_def a_def)
+    proof -
+      assume "pre4 s"
+      then have "s ''parv'' > 0"
+        unfolding pre4_def fAnd_def fGreater_def fLessEqual_def fOr_def fEqual_def fLess_def fNot_def
+        v_def evalE.simps by auto
+      then show "s ''parv'' * (1 / sqrt (s ''parv''))\<^sup>2 = 1"
+        by (smt divide_cancel_right nonzero_mult_div_cancel_left one_power2 power_divide
+                real_sqrt_pow2)
+    qed
+  qed
+   subgoal for s
+   proof -
+     have not_a: "not_in_fform ''para'' post4"
+       by(simp add:post4_def fAnd_def fGreaterEqual_def fLessEqual_def fOr_def fImp_def fEqual_def fLess_def fGreater_def fNot_def not_in_fform_def x_def y_def v_def dx_def dy_def)
+     have eq: "post4 (\<lambda>y. if y \<noteq> ''para'' then s y else 1 / sqrt (evalE v s)) \<longleftrightarrow> post4 s"
+      by (simp add: not_in_fform_update[OF not_a])
+    show ?thesis
+      apply (rule exI[where x="1/sqrt(evalE v s)"])
+      apply (auto simp add: eq fAnd_def fGreaterEqual_def fLessEqual_def fOr_def fImp_def fEqual_def fLess_def fGreater_def fNot_def  x_def y_def v_def a_def)
+    proof -
+      assume "post4 s"
+      then have "s ''parv'' > 0"
+        unfolding post4_def fAnd_def fGreater_def fLessEqual_def fOr_def fEqual_def fLess_def fNot_def
+        v_def evalE.simps by auto
+      then show "s ''parv'' * (1 / sqrt (s ''parv''))\<^sup>2 = 1"
+        by (smt divide_cancel_right nonzero_mult_div_cancel_left one_power2 power_divide
+                real_sqrt_pow2)
+    qed
+  qed
+  subgoal for h n d
+    apply(simp add:dOr_def almost_def fAnd_def a_def v_def)
+    apply (case_tac "n=d")
+    apply auto
+    apply (case_tac "n>d")
+     apply auto
+    apply (case_tac "n<d")
+     apply auto
+    apply (rule exI[where x="\<lambda>t y. 1/sqrt(evalE v (h t))"])
+    apply auto
+      apply (subgoal_tac "not_in_fform ''para'' post4")
+       apply(simp add:not_in_fform_def)
+       apply smt
+    apply(simp add:post4_def fAnd_def fGreaterEqual_def fLessEqual_def fOr_def fImp_def fEqual_def fLess_def fGreater_def fNot_def not_in_fform_def x_def y_def v_def dx_def dy_def)
+     apply(subgoal_tac"(h t ''parv'') > 0")
+      apply(simp add:fEqual_def v_def)
+    apply (simp add: power_divide)
+     apply(simp add:post4_def fAnd_def fGreaterEqual_def fLessEqual_def fOr_def fImp_def fEqual_def fLess_def fGreater_def fNot_def not_in_fform_def x_def y_def v_def dx_def dy_def)
+    apply auto
+    apply (subgoal_tac "not_in_fform ''para'' post4")
+       apply(simp add:not_in_fform_def)
+       apply smt
+    apply(simp add:post4_def fAnd_def fGreaterEqual_def fLessEqual_def fOr_def fImp_def fEqual_def fLess_def fGreater_def fNot_def not_in_fform_def x_def y_def v_def dx_def dy_def)
+    done
+  done
 
 definition pre5 :: fform where
-"pre5 == (Real g[\<ge>] Real 0)
+"pre5 == (Real g[>] Real 0)
       [&](v[>]Real 0)
-      [&](v[**]2 [+] Real (2*g) [*] y [=]Real (2*g*yG))
+      [&](v[**]2 [+] Real (2*g) [*] y [=]Real (v0^2)[+]Real (2*g*yG))
       [&]((Real dy0[\<ge>]Real 0 [&] x[\<le>]Real x1 [&] x[\<ge>]Real x0 [&] y[\<le>] Real y1 [&] y[\<ge>] Real y0)
          [\<longrightarrow>](((x[-]Real cx)[**]2[+](y[-]Real cy)[**]2) [=] Real r [**]2 [&] x[\<le>] Real cx[&] y[\<ge>] Real cy[&]v[**]2[\<ge>]Real vLo [&] v[**]2[\<le>]Real vHi [&] Real centLo[\<le>] Real cent[&]Real cent [\<le>]Real centHi [&] Real tanLo[\<le>]Real tan[&] Real tan[\<le>] Real tanHi))
       [&](Real dy0[\<ge>]Real 0)
-      [&](dx[=](y[-]Real cy)[div]Real r)
-      [&](dy[=](Real cx[-]x)[div]Real r)
+      [&](dx[*]Real r[=](y[-]Real cy))
+      [&](dy[*]Real r[=](Real cx[-]x))
       [&](Real x1[>]Real x0)
       [&](Real y1[>]Real y0)
       [&](Real cy[\<le>]Real y0)
       [&](Real x1[\<le>]Real cx)
       [&](Real r[>]Real 0)
-      [&]((x[\<le>]Real x1 [&] x[\<ge>]Real x0 [&] y[\<le>] Real y1 [&] y[\<ge>] Real y0)[\<longrightarrow>](v[**]2)[div]Real 2[>]Real g[*](Real y1[-]y))"
-
+      [&]((x[\<le>]Real x1 [&] x[\<ge>]Real x0 [&] y[\<le>] Real y1 [&] y[\<ge>] Real y0)[\<longrightarrow>](v[**]2)[div]Real 2[>]Real g[*](Real y1[-]y))
+      [&](x[\<le>]Real x1 [&] x[\<ge>]Real x0 [&] y[\<le>] Real y1 [&] y[\<ge>] Real y0)"
+     
 definition post5 :: fform where
-"post5 == (dx[=](y[-]Real cy)[div]Real r)
-       [&](dy[=](Real cx[-]x)[div]Real r)
+"post5 == (dx[*]Real r[=](y[-]Real cy))
+       [&](dy[*]Real r[=](Real cx[-]x))
        [&](v[>]Real 0)
-       [&](v[**]2 [+] Real (2*g) [*] y [=]Real (2*g*yG))
+       [&](v[**]2 [+] Real (2*g) [*] y [=]Real(v0^2)[+]Real (2*g*yG))
        [&](x[\<le>]Real cx)
        [&](Real cy[\<le>]y)
        [&](((x[-]Real cx)[**]2[+](y[-]Real cy)[**]2) [=] Real r [**]2)"
 
-definition Inv5 :: fform where
-"Inv5 == Inv"
+definition cons51 :: fform where
+"cons51 == pre5[&](v[*](a[**]2)[=]Real 1) [\<longrightarrow>] Inv"
+definition cons52 :: fform where
+"cons52 == Inv[&]close(x[\<le>]Real x1 [&] x[\<ge>]Real x0 [&] y[\<le>] Real y1 [&] y[\<ge>] Real y0)[\<longrightarrow>](post5[&](v[*](a[**]2)[=]Real 1))"
+definition cons53 :: fform where
+"cons53 == (exeFlow(<[''parx'',''pary'',''parv'',''pardx'',''pardy'',''para'']:[(v[*]dx),(v[*]dy),(dy[*]Real(-g)),((dy[*]v)[div]Real r),((Real 0[-]dx[*]v)[div]Real r),(((a[*]dy[*]Real g)[div](Real 2))[div]v)]&& Inv & (x[\<le>]Real x1 [&] x[\<ge>]Real x0 [&] y[\<le>] Real y1 [&] y[\<ge>] Real y0)>) (Inv)  [\<longrightarrow>]  Inv )"
+
+lemma allcons5:"\<forall>s. (cons51[&]cons52[&]cons53 ) s"
+  apply (simp add: cons51_def cons52_def cons53_def pre5_def post5_def x_def y_def v_def dx_def dy_def a_def)
+  by (inv_check_oracle "parv*(para^2)-1=0 & 
+                        parv>0 & 
+                        pardx*r-pary+cy=0 &
+                        pardy*r-cx+parx=0 &
+                        parv^2 + 2*g*pary -v0^2- 2*g*yG = 0 &
+                        (parx-cx)^2+(pary-cy)^2-r^2 = 0 &
+                        x1-cx<=0 &
+                        cy-y0<=0" "x1" "y0" )
+
+lemma q2le:"{pre5[&](v[*](a[**]2)[=]Real 1)}
+           <[''parx'',''pary'',''parv'',''pardx'',''pardy'',''para'']:[(v[*]dx),(v[*]dy),(dy[*]Real(-g)),((dy[*]v)[div]Real r),((Real 0[-]dx[*]v)[div]Real r),(((a[*]dy[*]Real g)[div](Real 2))[div]v)]&& Inv & (x[\<le>]Real x1 [&] x[\<ge>]Real x0 [&] y[\<le>] Real y1 [&] y[\<ge>] Real y0)>
+            {post5[&](v[*](a[**]2)[=]Real 1);(elE 0  [[|]] (almost (post5[&](v[*](a[**]2)[=]Real 1))))}"
+apply (rule ContinuousRuleGT )
+  apply auto
+       apply(simp add:pre5_def fAnd_def)
+      apply (cut_tac allcons5)
+      apply (simp add:cons51_def fAnd_def fImp_def)
+     apply (subgoal_tac "\<forall>s. cons52 s")
+      apply (simp add:cons52_def fImp_def )
+      apply (simp add:fAnd_def)
+     apply (cut_tac allcons5)
+     apply (simp add:fAnd_def )
+apply (cut_tac allcons5)
+    apply (simp add:cons53_def fAnd_def fImp_def)
+   apply (simp add:dOr_def)
+apply (subgoal_tac "\<forall>s. cons52 s")
+   apply (simp add:cons52_def fImp_def )
+   apply (simp add:dOr_def almost_def)
+ apply (cut_tac allcons5)
+  apply (simp add:fAnd_def )
+  done
+
 
 
 lemma q2:"{pre5}
-         <[''x'', ''y'', ''v'', ''dx'', ''dy'']: [(v[*]dx),(v[*]dy),(dy[*]Real -g),((dy[*]v)[div]Real r),((Real 0[-]dx[*]v)[div]Real r)] && Inv & (x[\<le>]Real x1 [&] x[\<ge>]Real x0 [&] y[\<le>] Real y1 [&] y[\<ge>] Real y0)>
+         <[''parx'', ''pary'', ''parv'', ''pardx'', ''pardy'']: [(v[*]dx),(v[*]dy),(dy[*]Real -g),((dy[*]v)[div]Real r),((Real 0[-]dx[*]v)[div]Real r)] && Inv & (x[\<le>]Real x1 [&] x[\<ge>]Real x0 [&] y[\<le>] Real y1 [&] y[\<ge>] Real y0)>
           {post5;(elE 0 [[|]] (almost post5))}"
-  sorry
+ apply (rule GhostRule[where w="''para''"
+                          and F="(((a[*]dy[*]Real g)[div](Real 2))[div]v)"
+                          and pre="pre5[&](v[*](a[**]2)[=]Real 1)"
+                          and post="post5[&](v[*](a[**]2)[=]Real 1)"
+                          and HF="(elE 0)[[|]]almost (post5[&](v[*](a[**]2)[=]Real 1))"])
+         apply auto
+  apply(simp add:pre5_def fAnd_def fGreaterEqual_def fLessEqual_def fOr_def fImp_def fEqual_def fLess_def fGreater_def fNot_def not_in_fform_def x_def y_def v_def dx_def dy_def)
+   apply(simp add:post5_def fAnd_def fGreaterEqual_def fLessEqual_def fOr_def fImp_def fEqual_def fLess_def fGreater_def fNot_def not_in_fform_def x_def y_def v_def dx_def dy_def) 
+  apply(simp add:dOr_def post5_def fAnd_def fGreaterEqual_def fLessEqual_def fOr_def fImp_def fEqual_def fLess_def fGreater_def fNot_def not_in_dform_def x_def y_def v_def dx_def dy_def almost_def)
+  apply(subgoal_tac "{pre5[&](v[*](a[**]2)[=]Real 1)}
+           <[''parx'',''pary'',''parv'',''pardx'',''pardy'',''para'']:[(v[*]dx),(v[*]dy),(dy[*]Real(-g)),((dy[*]v)[div]Real r),((Real 0[-]dx[*]v)[div]Real r),(((a[*]dy[*]Real g)[div](Real 2))[div]v)]&& Inv & (x[\<le>]Real x1 [&] x[\<ge>]Real x0 [&] y[\<le>] Real y1 [&] y[\<ge>] Real y0)>
+            {post5[&](v[*](a[**]2)[=]Real 1);(elE 0  [[|]] (almost (post5[&](v[*](a[**]2)[=]Real 1))))}")
+  apply(simp add: dOr_def)
+     apply (rule q2le)
+  subgoal for s
+  proof -
+    have not_a: "not_in_fform ''para'' pre5"
+      by (simp add:pre5_def fAnd_def fGreaterEqual_def fLessEqual_def fOr_def fImp_def fEqual_def fLess_def fGreater_def fNot_def not_in_fform_def x_def y_def v_def dx_def dy_def)
+    have eq: "pre5 (\<lambda>y. if y \<noteq> ''para'' then s y else 1 / sqrt (evalE v s)) \<longleftrightarrow> pre5 s"
+      by (simp add: not_in_fform_update[OF not_a])
+    show ?thesis
+      apply (rule exI[where x="1/sqrt(evalE v s)"])
+      apply (auto simp add: eq fAnd_def fGreaterEqual_def fLessEqual_def fOr_def fImp_def fEqual_def fLess_def fGreater_def fNot_def  x_def y_def v_def a_def)
+    proof -
+      assume "pre5 s"
+      then have "s ''parv'' > 0"
+        unfolding pre5_def fAnd_def fGreater_def fLessEqual_def fOr_def fEqual_def fLess_def fNot_def
+        v_def evalE.simps by auto
+      then show "s ''parv'' * (1 / sqrt (s ''parv''))\<^sup>2 = 1"
+        by (smt divide_cancel_right nonzero_mult_div_cancel_left one_power2 power_divide
+                real_sqrt_pow2)
+    qed
+  qed
+   subgoal for s
+   proof -
+     have not_a: "not_in_fform ''para'' post5"
+       by(simp add:post5_def fAnd_def fGreaterEqual_def fLessEqual_def fOr_def fImp_def fEqual_def fLess_def fGreater_def fNot_def not_in_fform_def x_def y_def v_def dx_def dy_def)
+     have eq: "post5 (\<lambda>y. if y \<noteq> ''para'' then s y else 1 / sqrt (evalE v s)) \<longleftrightarrow> post5 s"
+      by (simp add: not_in_fform_update[OF not_a])
+    show ?thesis
+      apply (rule exI[where x="1/sqrt(evalE v s)"])
+      apply (auto simp add: eq fAnd_def fGreaterEqual_def fLessEqual_def fOr_def fImp_def fEqual_def fLess_def fGreater_def fNot_def  x_def y_def v_def a_def)
+    proof -
+      assume "post5 s"
+      then have "s ''parv'' > 0"
+        unfolding post5_def fAnd_def fGreater_def fLessEqual_def fOr_def fEqual_def fLess_def fNot_def
+        v_def evalE.simps by auto
+      then show "s ''parv'' * (1 / sqrt (s ''parv''))\<^sup>2 = 1"
+        by (smt divide_cancel_right nonzero_mult_div_cancel_left one_power2 power_divide
+                real_sqrt_pow2)
+    qed
+  qed
+  subgoal for h n d
+    apply(simp add:dOr_def almost_def fAnd_def a_def v_def)
+    apply (case_tac "n=d")
+    apply auto
+    apply (case_tac "n>d")
+     apply auto
+    apply (case_tac "n<d")
+     apply auto
+    apply (rule exI[where x="\<lambda>t y. 1/sqrt(evalE v (h t))"])
+    apply auto
+      apply (subgoal_tac "not_in_fform ''para'' post5")
+       apply(simp add:not_in_fform_def)
+       apply smt
+    apply(simp add:post5_def fAnd_def fGreaterEqual_def fLessEqual_def fOr_def fImp_def fEqual_def fLess_def fGreater_def fNot_def not_in_fform_def x_def y_def v_def dx_def dy_def)
+     apply(subgoal_tac"(h t ''parv'') > 0")
+      apply(simp add:fEqual_def v_def)
+    apply (simp add: power_divide)
+     apply(simp add:post5_def fAnd_def fGreaterEqual_def fLessEqual_def fOr_def fImp_def fEqual_def fLess_def fGreater_def fNot_def not_in_fform_def x_def y_def v_def dx_def dy_def)
+    apply auto
+    apply (subgoal_tac "not_in_fform ''para'' post5")
+       apply(simp add:not_in_fform_def)
+       apply smt
+    apply(simp add:post5_def fAnd_def fGreaterEqual_def fLessEqual_def fOr_def fImp_def fEqual_def fLess_def fGreater_def fNot_def not_in_fform_def x_def y_def v_def dx_def dy_def)
+    done
+  done
 
+definition pre6 :: fform where
+"pre6 == (Real g[>] Real 0)
+      [&](v[>]Real 0)
+      [&](v[**]2 [+] Real (2*g) [*] y [=]Real (v0^2)[+]Real (2*g*yG))
+      [&]((Real dy0[\<le>]Real 0 [&] x[\<le>]Real x1 [&] x[\<ge>]Real x0 [&] y[\<le>] Real y0 [&] y[\<ge>] Real y1)
+         [\<longrightarrow>](((x[-]Real cx)[**]2[+](y[-]Real cy)[**]2) [=] Real r [**]2 [&] x[\<le>] Real cx[&] y[\<ge>] Real cy[&]v[**]2[\<ge>]Real vLo [&] v[**]2[\<le>]Real vHi [&] Real centLo[\<le>] Real cent[&]Real cent [\<le>]Real centHi [&] Real tanLo[\<le>]Real tan[&] Real tan[\<le>] Real tanHi))
+      [&](Real dy0[\<le>]Real 0)
+      [&](dx[*]Real r[=](Real cy[-]y))
+      [&](dy[*]Real r[=](x[-]Real cx))
+      [&](Real x1[>]Real x0)
+      [&](Real y1[<]Real y0)
+      [&](Real cy[\<le>]Real y1)
+      [&](Real x1[\<le>]Real cx)
+      [&](Real r[>]Real 0)
+      [&](x[\<le>]Real x1 [&] x[\<ge>]Real x0 [&] y[\<le>] Real y0 [&] y[\<ge>] Real y1)"
+     
+definition post6 :: fform where
+"post6 == (dx[*]Real r[=](Real cy[-]y))
+       [&](dy[*]Real r[=](x[-]Real cx))
+       [&](v[>]Real 0)
+       [&](v[**]2 [+] Real (2*g) [*] y [=]Real(v0^2)[+]Real (2*g*yG))
+       [&](x[\<le>]Real cx)
+       [&](Real cy[\<le>]y)
+       [&](((x[-]Real cx)[**]2[+](y[-]Real cy)[**]2) [=] Real r [**]2)"
+
+definition cons61 :: fform where
+"cons61 == pre6 [\<longrightarrow>] Inv"
+definition cons62 :: fform where
+"cons62 == Inv[&]close(x[\<le>]Real x1 [&] x[\<ge>]Real x0 [&] y[\<le>] Real y0 [&] y[\<ge>] Real y1)[\<longrightarrow>](post6)"
+definition cons63 :: fform where
+"cons63 == (exeFlow(<[''parx'',''pary'',''parv'',''pardx'',''pardy'']:[(v[*]dx),(v[*]dy),(dy[*]Real(-g)),((Real 0[-]dy[*]v)[div]Real r),((dx[*]v)[div]Real r)]&& Inv & (x[\<le>]Real x1 [&] x[\<ge>]Real x0 [&] y[\<le>] Real y0 [&] y[\<ge>] Real y1)>) (Inv)  [\<longrightarrow>]  Inv )"
+
+lemma allcons6:"\<forall>s. (cons61[&]cons62[&]cons63 ) s"
+  apply (simp add: cons61_def cons62_def cons63_def pre6_def post6_def x_def y_def v_def dx_def dy_def a_def)
+  by (inv_check_oracle "pardx*r-cy+pary=0 &
+                        pardy*r-parx+cx=0 &
+                        parv^2 + 2*g*pary -v0^2- 2*g*yG = 0 &
+                       (parx-cx)^2+(pary-cy)^2-r^2 = 0 &
+                        cx-x1>=0 &
+                        y1-cy>=0 &
+                        r>0 &
+                        g>0 &
+                        parv>0 " "x1" "y1")
+
+lemma q2cw:"{pre6}
+           <[''parx'',''pary'',''parv'',''pardx'',''pardy'']:[(v[*]dx),(v[*]dy),(dy[*]Real(-g)),((Real 0[-]dy[*]v)[div]Real r),((dx[*]v)[div]Real r)]&& Inv & (x[\<le>]Real x1 [&] x[\<ge>]Real x0 [&] y[\<le>] Real y0 [&] y[\<ge>] Real y1)>
+            {post6;(elE 0 [[|]] (almost post6))}"
+apply (rule ContinuousRuleGT )
+  apply auto
+       apply(simp add:pre6_def fAnd_def)
+      apply (cut_tac allcons6)
+      apply (simp add:cons61_def fAnd_def fImp_def)
+     apply (subgoal_tac "\<forall>s. cons62 s")
+      apply (simp add:cons62_def fImp_def )
+      apply (simp add:fAnd_def)
+     apply (cut_tac allcons6)
+     apply (simp add:fAnd_def )
+apply (cut_tac allcons6)
+    apply (simp add:cons63_def fAnd_def fImp_def)
+   apply (simp add:dOr_def)
+apply (subgoal_tac "\<forall>s. cons62 s")
+   apply (simp add:cons62_def fImp_def )
+   apply (simp add:dOr_def almost_def)
+ apply (cut_tac allcons6)
+  apply (simp add:fAnd_def )
+  done
+
+definition pre7 :: fform where
+"pre7 == (Real g[>] Real 0)
+      [&](v[>]Real 0)
+      [&](v[**]2 [+] Real (2*g) [*] y [=]Real (v0^2)[+]Real (2*g*yG))
+      [&]((Real dy0[\<le>]Real 0 [&] x[\<le>]Real x1 [&] x[\<ge>]Real x0 [&] y[\<le>] Real y0 [&] y[\<ge>] Real y1)
+         [\<longrightarrow>](((x[-]Real cx)[**]2[+](y[-]Real cy)[**]2) [=] Real r [**]2 [&] x[\<le>] Real cx[&] y[\<le>] Real cy[&]v[**]2[\<ge>]Real vLo [&] v[**]2[\<le>]Real vHi [&] Real centLo[\<le>] Real cent[&]Real cent [\<le>]Real centHi [&] Real tanLo[\<le>]Real tan[&] Real tan[\<le>] Real tanHi))
+      [&](Real dy0[\<le>]Real 0)
+      [&](dx[*]Real r[=](Real cy[-]y))
+      [&](dy[*]Real r[=](x[-]Real cx))
+      [&](Real x1[>]Real x0)
+      [&](Real y1[<]Real y0)
+      [&](Real cy[\<ge>]Real y0)
+      [&](Real x1[\<le>]Real cx)
+      [&](Real r[>]Real 0)
+      [&](x[\<le>]Real x1 [&] x[\<ge>]Real x0 [&] y[\<le>] Real y0 [&] y[\<ge>] Real y1)"
+     
+definition post7 :: fform where
+"post7 == (dx[*]Real r[=](Real cy[-]y))
+       [&](dy[*]Real r[=](x[-]Real cx))
+       [&](v[>]Real 0)
+       [&](v[**]2 [+] Real (2*g) [*] y [=]Real(v0^2)[+]Real (2*g*yG))
+       [&](x[\<le>]Real cx)
+       [&](Real cy[\<ge>]y)
+       [&](((x[-]Real cx)[**]2[+](y[-]Real cy)[**]2) [=] Real r [**]2)"
+
+definition cons71 :: fform where
+"cons71 == pre7 [\<longrightarrow>] Inv"
+definition cons72 :: fform where
+"cons72 == Inv[&]close(x[\<le>]Real x1 [&] x[\<ge>]Real x0 [&] y[\<le>] Real y0 [&] y[\<ge>] Real y1)[\<longrightarrow>](post7)"
+definition cons73 :: fform where
+"cons73 == (exeFlow(<[''parx'',''pary'',''parv'',''pardx'',''pardy'']:[(v[*]dx),(v[*]dy),(dy[*]Real(-g)),((Real 0[-]dy[*]v)[div]Real r),((dx[*]v)[div]Real r)]&& Inv & (x[\<le>]Real x1 [&] x[\<ge>]Real x0 [&] y[\<le>] Real y0 [&] y[\<ge>] Real y1)>) (Inv)  [\<longrightarrow>]  Inv )"
+
+lemma allcons7:"\<forall>s. (cons71[&]cons72[&]cons73 ) s"
+  apply (simp add: cons71_def cons72_def cons73_def pre7_def post7_def x_def y_def v_def dx_def dy_def a_def)
+  by (inv_check_oracle "pardx*r-cy+pary=0 &
+                        pardy*r-parx+cx=0 &
+                        parv^2 + 2*g*pary -v0^2- 2*g*yG = 0 &
+                       (parx-cx)^2+(pary-cy)^2-r^2 = 0 &
+                        cx-x1>=0 &
+                        cy-y0>=0 &
+                        r>0 &
+                        g>0 &
+                        parv>0 " "x1" "y0")
+
+lemma q3:"{pre7}
+           <[''parx'',''pary'',''parv'',''pardx'',''pardy'']:[(v[*]dx),(v[*]dy),(dy[*]Real(-g)),((Real 0[-]dy[*]v)[div]Real r),((dx[*]v)[div]Real r)]&& Inv & (x[\<le>]Real x1 [&] x[\<ge>]Real x0 [&] y[\<le>] Real y0 [&] y[\<ge>] Real y1)>
+            {post7;(elE 0 [[|]] (almost post7))}"
+apply (rule ContinuousRuleGT )
+  apply auto
+       apply(simp add:pre7_def fAnd_def)
+      apply (cut_tac allcons7)
+      apply (simp add:cons71_def fAnd_def fImp_def)
+     apply (subgoal_tac "\<forall>s. cons72 s")
+      apply (simp add:cons72_def fImp_def )
+      apply (simp add:fAnd_def)
+     apply (cut_tac allcons7)
+     apply (simp add:fAnd_def )
+apply (cut_tac allcons7)
+    apply (simp add:cons73_def fAnd_def fImp_def)
+   apply (simp add:dOr_def)
+apply (subgoal_tac "\<forall>s. cons72 s")
+   apply (simp add:cons72_def fImp_def )
+   apply (simp add:dOr_def almost_def)
+ apply (cut_tac allcons7)
+  apply (simp add:fAnd_def )
+  done
+
+
+
+
+definition pre8 :: fform where
+"pre8 == (Real g[>] Real 0)
+      [&](v[>]Real 0)
+      [&](v[**]2 [+] Real (2*g) [*] y [=]Real (v0^2)[+]Real (2*g*yG))
+      [&]((Real dy0[\<ge>]Real 0 [&] x[\<le>]Real x1 [&] x[\<ge>]Real x0 [&] y[\<le>] Real y1 [&] y[\<ge>] Real y0)
+         [\<longrightarrow>](((x[-]Real cx)[**]2[+](y[-]Real cy)[**]2) [=] Real r [**]2 [&] x[\<le>] Real cx[&] y[\<le>] Real cy[&]v[**]2[\<ge>]Real vLo [&] v[**]2[\<le>]Real vHi [&] Real centLo[\<le>] Real cent[&]Real cent [\<le>]Real centHi [&] Real tanLo[\<le>]Real tan[&] Real tan[\<le>] Real tanHi))
+      [&](Real dy0[\<ge>]Real 0)
+      [&](dx[*]Real r[=](y[-]Real cy))
+      [&](dy[*]Real r[=](Real cx[-]x))
+      [&](Real x1[>]Real x0)
+      [&](Real y1[>]Real y0)
+      [&](Real cy[\<ge>]Real y1)
+      [&](Real x1[\<le>]Real cx)
+      [&](Real r[>]Real 0)
+      [&]((x[\<le>]Real x1 [&] x[\<ge>]Real x0 [&] y[\<le>] Real y1 [&] y[\<ge>] Real y0)[\<longrightarrow>](v[**]2)[div]Real 2[>]Real g[*](Real y1[-]y))
+      [&](x[\<le>]Real x1 [&] x[\<ge>]Real x0 [&] y[\<le>] Real y1 [&] y[\<ge>] Real y0)"
+     
+definition post8 :: fform where
+"post8 == (dx[*]Real r[=](y[-]Real cy))
+       [&](dy[*]Real r[=](Real cx[-]x))
+       [&](v[>]Real 0)
+       [&](v[**]2 [+] Real (2*g) [*] y [=]Real(v0^2)[+]Real (2*g*yG))
+       [&](x[\<le>]Real cx)
+       [&](Real cy[\<ge>]y)
+       [&](((x[-]Real cx)[**]2[+](y[-]Real cy)[**]2) [=] Real r [**]2)"
+
+definition cons81 :: fform where
+"cons81 == pre8[&](v[*](a[**]2)[=]Real 1) [\<longrightarrow>] Inv"
+definition cons82 :: fform where
+"cons82 == Inv[&]close(x[\<le>]Real x1 [&] x[\<ge>]Real x0 [&] y[\<le>] Real y1 [&] y[\<ge>] Real y0)[\<longrightarrow>](post8[&](v[*](a[**]2)[=]Real 1))"
+definition cons83 :: fform where
+"cons83 == (exeFlow(<[''parx'',''pary'',''parv'',''pardx'',''pardy'',''para'']:[(v[*]dx),(v[*]dy),(dy[*]Real(-g)),((dy[*]v)[div]Real r),((Real 0[-]dx[*]v)[div]Real r),(((a[*]dy[*]Real g)[div](Real 2))[div]v)]&& Inv & (x[\<le>]Real x1 [&] x[\<ge>]Real x0 [&] y[\<le>] Real y1 [&] y[\<ge>] Real y0)>) (Inv)  [\<longrightarrow>]  Inv )"
+
+lemma allcons8:"\<forall>s. (cons81[&]cons82[&]cons83 ) s"
+  apply (simp add: cons81_def cons82_def cons83_def pre8_def post8_def x_def y_def v_def dx_def dy_def a_def)
+  by (inv_check_oracle "parv*(para^2)-1=0 & 
+                        parv>0 & 
+                        pardx*r-pary+cy=0 &
+                        pardy*r-cx+parx=0 &
+                        parv^2 + 2*g*pary -v0^2- 2*g*yG = 0 &
+                        (parx-cx)^2+(pary-cy)^2-r^2 = 0 &
+                        x1-cx<=0 &
+                        cy-y1>=0" "x1" "y1" )
+
+lemma q3cwle:"{pre8[&](v[*](a[**]2)[=]Real 1)}
+           <[''parx'',''pary'',''parv'',''pardx'',''pardy'',''para'']:[(v[*]dx),(v[*]dy),(dy[*]Real(-g)),((dy[*]v)[div]Real r),((Real 0[-]dx[*]v)[div]Real r),(((a[*]dy[*]Real g)[div](Real 2))[div]v)]&& Inv & (x[\<le>]Real x1 [&] x[\<ge>]Real x0 [&] y[\<le>] Real y1 [&] y[\<ge>] Real y0)>
+            {post8[&](v[*](a[**]2)[=]Real 1);(elE 0  [[|]] (almost (post8[&](v[*](a[**]2)[=]Real 1))))}"
+apply (rule ContinuousRuleGT )
+  apply auto
+       apply(simp add:pre8_def fAnd_def)
+      apply (cut_tac allcons8)
+      apply (simp add:cons81_def fAnd_def fImp_def)
+     apply (subgoal_tac "\<forall>s. cons82 s")
+      apply (simp add:cons82_def fImp_def )
+      apply (simp add:fAnd_def)
+     apply (cut_tac allcons8)
+     apply (simp add:fAnd_def )
+apply (cut_tac allcons8)
+    apply (simp add:cons83_def fAnd_def fImp_def)
+   apply (simp add:dOr_def)
+apply (subgoal_tac "\<forall>s. cons82 s")
+   apply (simp add:cons82_def fImp_def )
+   apply (simp add:dOr_def almost_def)
+ apply (cut_tac allcons8)
+  apply (simp add:fAnd_def )
+  done
+
+
+
+lemma q3cw:"{pre8}
+         <[''parx'', ''pary'', ''parv'', ''pardx'', ''pardy'']: [(v[*]dx),(v[*]dy),(dy[*]Real -g),((dy[*]v)[div]Real r),((Real 0[-]dx[*]v)[div]Real r)] && Inv & (x[\<le>]Real x1 [&] x[\<ge>]Real x0 [&] y[\<le>] Real y1 [&] y[\<ge>] Real y0)>
+          {post8;(elE 0 [[|]] (almost post8))}"
+ apply (rule GhostRule[where w="''para''"
+                          and F="(((a[*]dy[*]Real g)[div](Real 2))[div]v)"
+                          and pre="pre8[&](v[*](a[**]2)[=]Real 1)"
+                          and post="post8[&](v[*](a[**]2)[=]Real 1)"
+                          and HF="(elE 0)[[|]]almost (post8[&](v[*](a[**]2)[=]Real 1))"])
+         apply auto
+  apply(simp add:pre8_def fAnd_def fGreaterEqual_def fLessEqual_def fOr_def fImp_def fEqual_def fLess_def fGreater_def fNot_def not_in_fform_def x_def y_def v_def dx_def dy_def)
+   apply(simp add:post8_def fAnd_def fGreaterEqual_def fLessEqual_def fOr_def fImp_def fEqual_def fLess_def fGreater_def fNot_def not_in_fform_def x_def y_def v_def dx_def dy_def) 
+  apply(simp add:dOr_def post8_def fAnd_def fGreaterEqual_def fLessEqual_def fOr_def fImp_def fEqual_def fLess_def fGreater_def fNot_def not_in_dform_def x_def y_def v_def dx_def dy_def almost_def)
+  apply(subgoal_tac "{pre8[&](v[*](a[**]2)[=]Real 1)}
+           <[''parx'',''pary'',''parv'',''pardx'',''pardy'',''para'']:[(v[*]dx),(v[*]dy),(dy[*]Real(-g)),((dy[*]v)[div]Real r),((Real 0[-]dx[*]v)[div]Real r),(((a[*]dy[*]Real g)[div](Real 2))[div]v)]&& Inv & (x[\<le>]Real x1 [&] x[\<ge>]Real x0 [&] y[\<le>] Real y1 [&] y[\<ge>] Real y0)>
+            {post8[&](v[*](a[**]2)[=]Real 1);(elE 0  [[|]] (almost (post8[&](v[*](a[**]2)[=]Real 1))))}")
+  apply(simp add: dOr_def)
+     apply (rule q3cwle)
+  subgoal for s
+  proof -
+    have not_a: "not_in_fform ''para'' pre8"
+      by (simp add:pre8_def fAnd_def fGreaterEqual_def fLessEqual_def fOr_def fImp_def fEqual_def fLess_def fGreater_def fNot_def not_in_fform_def x_def y_def v_def dx_def dy_def)
+    have eq: "pre8 (\<lambda>y. if y \<noteq> ''para'' then s y else 1 / sqrt (evalE v s)) \<longleftrightarrow> pre8 s"
+      by (simp add: not_in_fform_update[OF not_a])
+    show ?thesis
+      apply (rule exI[where x="1/sqrt(evalE v s)"])
+      apply (auto simp add: eq fAnd_def fGreaterEqual_def fLessEqual_def fOr_def fImp_def fEqual_def fLess_def fGreater_def fNot_def  x_def y_def v_def a_def)
+    proof -
+      assume "pre8 s"
+      then have "s ''parv'' > 0"
+        unfolding pre8_def fAnd_def fGreater_def fLessEqual_def fOr_def fEqual_def fLess_def fNot_def
+        v_def evalE.simps by auto
+      then show "s ''parv'' * (1 / sqrt (s ''parv''))\<^sup>2 = 1"
+        by (smt divide_cancel_right nonzero_mult_div_cancel_left one_power2 power_divide
+                real_sqrt_pow2)
+    qed
+  qed
+   subgoal for s
+   proof -
+     have not_a: "not_in_fform ''para'' post8"
+       by(simp add:post8_def fAnd_def fGreaterEqual_def fLessEqual_def fOr_def fImp_def fEqual_def fLess_def fGreater_def fNot_def not_in_fform_def x_def y_def v_def dx_def dy_def)
+     have eq: "post8 (\<lambda>y. if y \<noteq> ''para'' then s y else 1 / sqrt (evalE v s)) \<longleftrightarrow> post8 s"
+      by (simp add: not_in_fform_update[OF not_a])
+    show ?thesis
+      apply (rule exI[where x="1/sqrt(evalE v s)"])
+      apply (auto simp add: eq fAnd_def fGreaterEqual_def fLessEqual_def fOr_def fImp_def fEqual_def fLess_def fGreater_def fNot_def  x_def y_def v_def a_def)
+    proof -
+      assume "post8 s"
+      then have "s ''parv'' > 0"
+        unfolding post8_def fAnd_def fGreater_def fLessEqual_def fOr_def fEqual_def fLess_def fNot_def
+        v_def evalE.simps by auto
+      then show "s ''parv'' * (1 / sqrt (s ''parv''))\<^sup>2 = 1"
+        by (smt divide_cancel_right nonzero_mult_div_cancel_left one_power2 power_divide
+                real_sqrt_pow2)
+    qed
+  qed
+  subgoal for h n d
+    apply(simp add:dOr_def almost_def fAnd_def a_def v_def)
+    apply (case_tac "n=d")
+    apply auto
+    apply (case_tac "n>d")
+     apply auto
+    apply (case_tac "n<d")
+     apply auto
+    apply (rule exI[where x="\<lambda>t y. 1/sqrt(evalE v (h t))"])
+    apply auto
+      apply (subgoal_tac "not_in_fform ''para'' post8")
+       apply(simp add:not_in_fform_def)
+       apply smt
+    apply(simp add:post8_def fAnd_def fGreaterEqual_def fLessEqual_def fOr_def fImp_def fEqual_def fLess_def fGreater_def fNot_def not_in_fform_def x_def y_def v_def dx_def dy_def)
+     apply(subgoal_tac"(h t ''parv'') > 0")
+      apply(simp add:fEqual_def v_def)
+    apply (simp add: power_divide)
+     apply(simp add:post8_def fAnd_def fGreaterEqual_def fLessEqual_def fOr_def fImp_def fEqual_def fLess_def fGreater_def fNot_def not_in_fform_def x_def y_def v_def dx_def dy_def)
+    apply auto
+    apply (subgoal_tac "not_in_fform ''para'' post8")
+       apply(simp add:not_in_fform_def)
+       apply smt
+    apply(simp add:post8_def fAnd_def fGreaterEqual_def fLessEqual_def fOr_def fImp_def fEqual_def fLess_def fGreater_def fNot_def not_in_fform_def x_def y_def v_def dx_def dy_def)
+    done
+  done
+
+
+definition pre9 :: fform where
+"pre9 == (Real g[>] Real 0)
+      [&](v[>]Real 0)
+      [&](v[**]2 [+] Real (2*g) [*] y [=]Real (v0^2)[+]Real (2*g*yG))
+      [&]((Real dy0[\<ge>]Real 0 [&] x[\<le>]Real x1 [&] x[\<ge>]Real x0 [&] y[\<le>] Real y1 [&] y[\<ge>] Real y0)
+         [\<longrightarrow>](((x[-]Real cx)[**]2[+](y[-]Real cy)[**]2) [=] Real r [**]2 [&] x[\<ge>] Real cx[&] y[\<le>] Real cy[&]v[**]2[\<ge>]Real vLo [&] v[**]2[\<le>]Real vHi [&] Real centLo[\<le>] Real cent[&]Real cent [\<le>]Real centHi [&] Real tanLo[\<le>]Real tan[&] Real tan[\<le>] Real tanHi))
+      [&](Real dy0[\<ge>]Real 0)
+      [&](dx[*]Real r[=](Real cy[-]y))
+      [&](dy[*]Real r[=](x[-]Real cx))
+      [&](Real x1[>]Real x0)
+      [&](Real y1[>]Real y0)
+      [&](Real cy[\<ge>]Real y1)
+      [&](Real x0[\<ge>]Real cx)
+      [&](Real r[>]Real 0)
+      [&]((x[\<le>]Real x1 [&] x[\<ge>]Real x0 [&] y[\<le>] Real y1 [&] y[\<ge>] Real y0)[\<longrightarrow>](v[**]2)[div]Real 2[>]Real g[*](Real y1[-]y))
+      [&](x[\<le>]Real x1 [&] x[\<ge>]Real x0 [&] y[\<le>] Real y1 [&] y[\<ge>] Real y0)"
+     
+definition post9 :: fform where
+"post9 == (dx[*]Real r[=](Real cy[-]y))
+       [&](dy[*]Real r[=](x[-]Real cx))
+       [&](v[>]Real 0)
+       [&](v[**]2 [+] Real (2*g) [*] y [=]Real(v0^2)[+]Real (2*g*yG))
+       [&](x[\<ge>]Real cx)
+       [&](Real cy[\<ge>]y)
+       [&](((x[-]Real cx)[**]2[+](y[-]Real cy)[**]2) [=] Real r [**]2)"
+
+definition cons91 :: fform where
+"cons91 == pre9[&](v[*](a[**]2)[=]Real 1) [\<longrightarrow>] Inv"
+definition cons92 :: fform where
+"cons92 == Inv[&]close(x[\<le>]Real x1 [&] x[\<ge>]Real x0 [&] y[\<le>] Real y1 [&] y[\<ge>] Real y0)[\<longrightarrow>](post9[&](v[*](a[**]2)[=]Real 1))"
+definition cons93 :: fform where
+"cons93 == (exeFlow(<[''parx'',''pary'',''parv'',''pardx'',''pardy'',''para'']:[(v[*]dx),(v[*]dy),(dy[*]Real(-g)),((Real 0[-]dy[*]v)[div]Real r),((dx[*]v)[div]Real r),(((a[*]dy[*]Real g)[div](Real 2))[div]v)]&& Inv & (x[\<le>]Real x1 [&] x[\<ge>]Real x0 [&] y[\<le>] Real y1 [&] y[\<ge>] Real y0)>) (Inv)  [\<longrightarrow>]  Inv )"
+
+lemma allcons9:"\<forall>s. (cons91[&]cons92[&]cons93 ) s"
+  apply (simp add: cons91_def cons92_def cons93_def pre9_def post9_def x_def y_def v_def dx_def dy_def a_def)
+  by (inv_check_oracle "parv*(para^2)-1=0 & 
+                        parv>0 & 
+                        pardx*r+pary-cy=0 &
+                        pardy*r+cx-parx=0 &
+                        parv^2 + 2*g*pary -v0^2- 2*g*yG = 0 &
+                        (parx-cx)^2+(pary-cy)^2-r^2 = 0 &
+                        x0-cx>=0 &
+                        cy-y1>=0" "x0" "y1" )
+
+lemma q4le:"{pre9[&](v[*](a[**]2)[=]Real 1)}
+           <[''parx'',''pary'',''parv'',''pardx'',''pardy'',''para'']:[(v[*]dx),(v[*]dy),(dy[*]Real(-g)),((Real 0[-]dy[*]v)[div]Real r),((dx[*]v)[div]Real r),(((a[*]dy[*]Real g)[div](Real 2))[div]v)]&& Inv & (x[\<le>]Real x1 [&] x[\<ge>]Real x0 [&] y[\<le>] Real y1 [&] y[\<ge>] Real y0)>
+            {post9[&](v[*](a[**]2)[=]Real 1);(elE 0  [[|]] (almost (post9[&](v[*](a[**]2)[=]Real 1))))}"
+apply (rule ContinuousRuleGT )
+  apply auto
+       apply(simp add:pre9_def fAnd_def)
+      apply (cut_tac allcons9)
+      apply (simp add:cons91_def fAnd_def fImp_def)
+     apply (subgoal_tac "\<forall>s. cons92 s")
+      apply (simp add:cons92_def fImp_def )
+      apply (simp add:fAnd_def)
+     apply (cut_tac allcons9)
+     apply (simp add:fAnd_def )
+apply (cut_tac allcons9)
+    apply (simp add:cons93_def fAnd_def fImp_def)
+   apply (simp add:dOr_def)
+apply (subgoal_tac "\<forall>s. cons92 s")
+   apply (simp add:cons92_def fImp_def )
+   apply (simp add:dOr_def almost_def)
+ apply (cut_tac allcons9)
+  apply (simp add:fAnd_def )
+  done
+
+
+
+lemma q4:"{pre9}
+         <[''parx'', ''pary'', ''parv'', ''pardx'', ''pardy'']: [(v[*]dx),(v[*]dy),(dy[*]Real -g),((Real 0[-]dy[*]v)[div]Real r),((dx[*]v)[div]Real r)] && Inv & (x[\<le>]Real x1 [&] x[\<ge>]Real x0 [&] y[\<le>] Real y1 [&] y[\<ge>] Real y0)>
+          {post9;(elE 0 [[|]] (almost post9))}"
+ apply (rule GhostRule[where w="''para''"
+                          and F="(((a[*]dy[*]Real g)[div](Real 2))[div]v)"
+                          and pre="pre9[&](v[*](a[**]2)[=]Real 1)"
+                          and post="post9[&](v[*](a[**]2)[=]Real 1)"
+                          and HF="(elE 0)[[|]]almost (post9[&](v[*](a[**]2)[=]Real 1))"])
+         apply auto
+  apply(simp add:pre9_def fAnd_def fGreaterEqual_def fLessEqual_def fOr_def fImp_def fEqual_def fLess_def fGreater_def fNot_def not_in_fform_def x_def y_def v_def dx_def dy_def)
+   apply(simp add:post9_def fAnd_def fGreaterEqual_def fLessEqual_def fOr_def fImp_def fEqual_def fLess_def fGreater_def fNot_def not_in_fform_def x_def y_def v_def dx_def dy_def) 
+  apply(simp add:dOr_def post9_def fAnd_def fGreaterEqual_def fLessEqual_def fOr_def fImp_def fEqual_def fLess_def fGreater_def fNot_def not_in_dform_def x_def y_def v_def dx_def dy_def almost_def)
+  apply(subgoal_tac "{pre9[&](v[*](a[**]2)[=]Real 1)}
+           <[''parx'',''pary'',''parv'',''pardx'',''pardy'',''para'']:[(v[*]dx),(v[*]dy),(dy[*]Real(-g)),((Real 0[-]dy[*]v)[div]Real r),((dx[*]v)[div]Real r),(((a[*]dy[*]Real g)[div](Real 2))[div]v)]&& Inv & (x[\<le>]Real x1 [&] x[\<ge>]Real x0 [&] y[\<le>] Real y1 [&] y[\<ge>] Real y0)>
+            {post9[&](v[*](a[**]2)[=]Real 1);(elE 0  [[|]] (almost (post9[&](v[*](a[**]2)[=]Real 1))))}")
+  apply(simp add: dOr_def)
+     apply (rule q4le)
+  subgoal for s
+  proof -
+    have not_a: "not_in_fform ''para'' pre9"
+      by (simp add:pre9_def fAnd_def fGreaterEqual_def fLessEqual_def fOr_def fImp_def fEqual_def fLess_def fGreater_def fNot_def not_in_fform_def x_def y_def v_def dx_def dy_def)
+    have eq: "pre9 (\<lambda>y. if y \<noteq> ''para'' then s y else 1 / sqrt (evalE v s)) \<longleftrightarrow> pre9 s"
+      by (simp add: not_in_fform_update[OF not_a])
+    show ?thesis
+      apply (rule exI[where x="1/sqrt(evalE v s)"])
+      apply (auto simp add: eq fAnd_def fGreaterEqual_def fLessEqual_def fOr_def fImp_def fEqual_def fLess_def fGreater_def fNot_def  x_def y_def v_def a_def)
+    proof -
+      assume "pre9 s"
+      then have "s ''parv'' > 0"
+        unfolding pre9_def fAnd_def fGreater_def fLessEqual_def fOr_def fEqual_def fLess_def fNot_def
+        v_def evalE.simps by auto
+      then show "s ''parv'' * (1 / sqrt (s ''parv''))\<^sup>2 = 1"
+        by (smt divide_cancel_right nonzero_mult_div_cancel_left one_power2 power_divide
+                real_sqrt_pow2)
+    qed
+  qed
+   subgoal for s
+   proof -
+     have not_a: "not_in_fform ''para'' post9"
+       by(simp add:post9_def fAnd_def fGreaterEqual_def fLessEqual_def fOr_def fImp_def fEqual_def fLess_def fGreater_def fNot_def not_in_fform_def x_def y_def v_def dx_def dy_def)
+     have eq: "post9 (\<lambda>y. if y \<noteq> ''para'' then s y else 1 / sqrt (evalE v s)) \<longleftrightarrow> post9 s"
+      by (simp add: not_in_fform_update[OF not_a])
+    show ?thesis
+      apply (rule exI[where x="1/sqrt(evalE v s)"])
+      apply (auto simp add: eq fAnd_def fGreaterEqual_def fLessEqual_def fOr_def fImp_def fEqual_def fLess_def fGreater_def fNot_def  x_def y_def v_def a_def)
+    proof -
+      assume "post9 s"
+      then have "s ''parv'' > 0"
+        unfolding post9_def fAnd_def fGreater_def fLessEqual_def fOr_def fEqual_def fLess_def fNot_def
+        v_def evalE.simps by auto
+      then show "s ''parv'' * (1 / sqrt (s ''parv''))\<^sup>2 = 1"
+        by (smt divide_cancel_right nonzero_mult_div_cancel_left one_power2 power_divide
+                real_sqrt_pow2)
+    qed
+  qed
+  subgoal for h n d
+    apply(simp add:dOr_def almost_def fAnd_def a_def v_def)
+    apply (case_tac "n=d")
+    apply auto
+    apply (case_tac "n>d")
+     apply auto
+    apply (case_tac "n<d")
+     apply auto
+    apply (rule exI[where x="\<lambda>t y. 1/sqrt(evalE v (h t))"])
+    apply auto
+      apply (subgoal_tac "not_in_fform ''para'' post9")
+       apply(simp add:not_in_fform_def)
+       apply smt
+    apply(simp add:post9_def fAnd_def fGreaterEqual_def fLessEqual_def fOr_def fImp_def fEqual_def fLess_def fGreater_def fNot_def not_in_fform_def x_def y_def v_def dx_def dy_def)
+     apply(subgoal_tac"(h t ''parv'') > 0")
+      apply(simp add:fEqual_def v_def)
+    apply (simp add: power_divide)
+     apply(simp add:post9_def fAnd_def fGreaterEqual_def fLessEqual_def fOr_def fImp_def fEqual_def fLess_def fGreater_def fNot_def not_in_fform_def x_def y_def v_def dx_def dy_def)
+    apply auto
+    apply (subgoal_tac "not_in_fform ''para'' post9")
+       apply(simp add:not_in_fform_def)
+       apply smt
+    apply(simp add:post9_def fAnd_def fGreaterEqual_def fLessEqual_def fOr_def fImp_def fEqual_def fLess_def fGreater_def fNot_def not_in_fform_def x_def y_def v_def dx_def dy_def)
+    done
+  done
+definition pre10 :: fform where
+"pre10 == (Real g[>] Real 0)
+      [&](v[>]Real 0)
+      [&](v[**]2 [+] Real (2*g) [*] y [=]Real (v0^2)[+]Real (2*g*yG))
+      [&]((Real dy0[\<le>]Real 0 [&] x[\<le>]Real x1 [&] x[\<ge>]Real x0 [&] y[\<le>] Real y1 [&] y[\<ge>] Real y0)
+         [\<longrightarrow>](((x[-]Real cx)[**]2[+](y[-]Real cy)[**]2) [=] Real r [**]2 [&] x[\<ge>] Real cx[&] y[\<le>] Real cy[&]v[**]2[\<ge>]Real vLo [&] v[**]2[\<le>]Real vHi [&] Real centLo[\<le>] Real cent[&]Real cent [\<le>]Real centHi [&] Real tanLo[\<le>]Real tan[&] Real tan[\<le>] Real tanHi))
+      [&](Real dy0[\<le>]Real 0)
+      [&](dx[*]Real r[=](y[-]Real cy))
+      [&](dy[*]Real r[=](Real cx[-]x))
+      [&](Real x1[>]Real x0)
+      [&](Real y1[>]Real y0)
+      [&](Real cy[\<ge>]Real y1)
+      [&](Real x0[\<ge>]Real cx)
+      [&](Real r[>]Real 0)
+      [&](x[\<le>]Real x1 [&] x[\<ge>]Real x0 [&] y[\<le>] Real y1 [&] y[\<ge>] Real y0)"
+     
+definition post10 :: fform where
+"post10 == (dx[*]Real r[=](y[-]Real cy))
+       [&](dy[*]Real r[=](Real cx[-]x))
+       [&](v[>]Real 0)
+       [&](v[**]2 [+] Real (2*g) [*] y [=]Real(v0^2)[+]Real (2*g*yG))
+       [&](x[\<ge>]Real cx)
+       [&](Real cy[\<ge>]y)
+       [&](((x[-]Real cx)[**]2[+](y[-]Real cy)[**]2) [=] Real r [**]2)"
+
+definition cons101 :: fform where
+"cons101 == pre10 [\<longrightarrow>] Inv"
+definition cons102 :: fform where
+"cons102 == Inv[&]close(x[\<le>]Real x1 [&] x[\<ge>]Real x0 [&] y[\<le>] Real y1 [&] y[\<ge>] Real y0)[\<longrightarrow>](post10)"
+definition cons103 :: fform where
+"cons103 == (exeFlow(<[''parx'',''pary'',''parv'',''pardx'',''pardy'']:[(v[*]dx),(v[*]dy),(dy[*]Real(-g)),((dy[*]v)[div]Real r),((Real 0[-]dx[*]v)[div]Real r)]&& Inv & (x[\<le>]Real x1 [&] x[\<ge>]Real x0 [&] y[\<le>] Real y1 [&] y[\<ge>] Real y0)>) (Inv)  [\<longrightarrow>]  Inv )"
+
+lemma allcons10:"\<forall>s. (cons101[&]cons102[&]cons103 ) s"
+  apply (simp add: cons101_def cons102_def cons103_def pre10_def post10_def x_def y_def v_def dx_def dy_def a_def)
+  by (inv_check_oracle "pardx*r+cy-pary=0 &
+                        pardy*r+parx-cx=0 &
+                        parv^2 + 2*g*pary -v0^2- 2*g*yG = 0 &
+                       (parx-cx)^2+(pary-cy)^2-r^2 = 0 &
+                        cx-x0<=0 &
+                        cy-y1>=0 &
+                        r>0 &
+                        g>0 &
+                        parv>0 " "x0" "y1")
+
+lemma q4cw:"{pre10}
+           <[''parx'',''pary'',''parv'',''pardx'',''pardy'']:[(v[*]dx),(v[*]dy),(dy[*]Real(-g)),((dy[*]v)[div]Real r),((Real 0[-]dx[*]v)[div]Real r)]&& Inv & (x[\<le>]Real x1 [&] x[\<ge>]Real x0 [&] y[\<le>] Real y1 [&] y[\<ge>] Real y0)>
+            {post10;(elE 0 [[|]] (almost post10))}"
+apply (rule ContinuousRuleGT )
+  apply auto
+       apply(simp add:pre10_def fAnd_def)
+      apply (cut_tac allcons10)
+      apply (simp add:cons101_def fAnd_def fImp_def)
+     apply (subgoal_tac "\<forall>s. cons102 s")
+      apply (simp add:cons102_def fImp_def )
+      apply (simp add:fAnd_def)
+     apply (cut_tac allcons10)
+     apply (simp add:fAnd_def )
+apply (cut_tac allcons10)
+    apply (simp add:cons103_def fAnd_def fImp_def)
+   apply (simp add:dOr_def)
+apply (subgoal_tac "\<forall>s. cons102 s")
+   apply (simp add:cons102_def fImp_def )
+   apply (simp add:dOr_def almost_def)
+ apply (cut_tac allcons10)
+  apply (simp add:fAnd_def )
+  done
 
 
 
